refactor: bundle `Op` and `Ty` into a `Dialect` struct
The diff is rather huge, but the change is almost completely mechanical, using find/replace

SSA/Core/Framework.lean
@@ -15,6 +15,11 @@ open TyDenote (toType)
   # Classes
 -/
 
+/-- A MLIR `Dialect` is comprised of a type of `Op`erations, and a type of `Ty`pes -/
+structure Dialect where
+  Op : Type
+  Ty : Type
+
 abbrev RegionSignature Ty := List (Ctxt Ty × Ty)
 
 structure Signature (Ty : Type) where
@@ -22,12 +27,12 @@ structure Signature (Ty : Type) where
   regSig  : RegionSignature Ty
   outTy   : Ty
 
-class OpSignature (Op : Type) (Ty : outParam (Type)) where
-  signature : Op → Signature Ty
+class OpSignature (d : Dialect) where
+  signature : d.Op → Signature d.Ty
 export OpSignature (signature)
 
 section
-variable {Op Ty} [s : OpSignature Op Ty]
+variable {d} [s : OpSignature d]
 
 def OpSignature.sig     := Signature.sig ∘ s.signature
 def OpSignature.regSig  := Signature.regSig ∘ s.signature
@@ -36,29 +41,29 @@ def OpSignature.outTy   := Signature.outTy ∘ s.signature
 end
 
 
-class OpDenote (Op Ty : Type) [TyDenote Ty] [OpSignature Op Ty] where
-  denote : (op : Op) → HVector toType (OpSignature.sig op) →
-    HVector (fun t : Ctxt Ty × Ty => t.1.Valuation → toType t.2) (OpSignature.regSig op) →
+class OpDenote (d : Dialect) [TyDenote d.Ty] [OpSignature d] where
+  denote : (op : d.Op) → HVector toType (OpSignature.sig op) →
+    HVector (fun t : Ctxt d.Ty × d.Ty => t.1.Valuation → toType t.2) (OpSignature.regSig op) →
     (toType <| OpSignature.outTy op)
 
 /-
   # Datastructures
 -/
 
-variable (Op : Type) {Ty : Type} [OpSignature Op Ty]
+variable (d : Dialect) [OpSignature d]
 
 mutual
 
 /-- A very simple intrinsically typed expression. -/
-inductive Expr : (Γ : Ctxt Ty) → (ty : Ty) → Type :=
-  | mk {Γ} {ty} (op : Op)
+inductive Expr : (Γ : Ctxt d.Ty) → (ty : d.Ty) → Type :=
+  | mk {Γ} {ty} (op : d.Op)
     (ty_eq : ty = OpSignature.outTy op)
     (args : HVector (Var Γ) <| OpSignature.sig op)
-    (regArgs : HVector (fun t : Ctxt Ty × Ty => Com t.1 t.2)
+    (regArgs : HVector (fun t : Ctxt d.Ty × d.Ty => Com t.1 t.2)
       (OpSignature.regSig op)) : Expr Γ ty
 
 /-- A very simple intrinsically typed program: a sequence of let bindings. -/
-inductive Com : Ctxt Ty → Ty → Type where
+inductive Com : Ctxt d.Ty → d.Ty → Type where
   | ret (v : Var Γ t) : Com Γ t
   | lete (e : Expr Γ α) (body : Com (Γ.snoc α) β) : Com Γ β
 
@@ -66,35 +71,37 @@ end
 
 section
 open Std (Format)
-variable {Op Ty : Type} [OpSignature Op Ty] [Repr Op] [Repr Ty]
+variable {d} [OpSignature d] [Repr d.Op] [Repr d.Ty]
 
 mutual
-  def Expr.repr (prec : Nat) : Expr Op Γ t → Format
+  def Expr.repr (prec : Nat) : Expr d Γ t → Format
     | ⟨op, _, args, _regArgs⟩ => f!"{repr op}{repr args}"
 
-  def Com.repr (prec : Nat) : Com Op Γ t → Format
+  def Com.repr (prec : Nat) : Com d Γ t → Format
     | .ret v => .align false ++ f!"return {reprPrec v prec}"
     | .lete e body => (.align false ++ f!"{e.repr prec}") ++ body.repr prec
 end
 
-instance : Repr (Expr Op Γ t) := ⟨flip Expr.repr⟩
-instance : Repr (Com Op Γ t) := ⟨flip Com.repr⟩
+instance : Repr (Expr d Γ t) := ⟨flip Expr.repr⟩
+instance : Repr (Com d Γ t) := ⟨flip Com.repr⟩
 
 end
 
 --TODO: this should be derived later on when a derive handler is implemented
 mutual
 
-protected instance HVector.decidableEqReg [DecidableEq Op] [DecidableEq Ty] :
-    ∀ {l : List (Ctxt Ty × Ty)}, DecidableEq (HVector (fun t => Com Op t.1 t.2) l)
+variable {d} [OpSignature d]
+
+protected instance HVector.decidableEqReg [DecidableEq d.Op] [DecidableEq d.Ty] :
+    ∀ {l : List (Ctxt d.Ty × d.Ty)}, DecidableEq (HVector (fun t => Com d t.1 t.2) l)
   | _, .nil, .nil => isTrue rfl
   | _, .cons x₁ v₁, .cons x₂ v₂ =>
     letI := HVector.decidableEqReg v₁ v₂
     letI := Com.decidableEq x₁ x₂
     decidable_of_iff (x₁ = x₂ ∧ v₁ = v₂) (by simp)
 
-protected instance Expr.decidableEq [DecidableEq Op] [DecidableEq Ty] :
-    {Γ : Ctxt Ty} → {ty : Ty} → DecidableEq (Expr Op Γ ty)
+protected instance Expr.decidableEq [DecidableEq d.Op] [DecidableEq d.Ty] :
+    {Γ : Ctxt d.Ty} → {ty : d.Ty} → DecidableEq (Expr d Γ ty)
   | _, _, .mk op₁ rfl arg₁ regArgs₁, .mk op₂ eq arg₂ regArgs₂ =>
     if ho : op₁ = op₂
     then by
@@ -104,8 +111,8 @@ protected instance Expr.decidableEq [DecidableEq Op] [DecidableEq Ty] :
       exact decidable_of_iff (arg₁ = arg₂ ∧ regArgs₁ = regArgs₂) (by simp)
     else isFalse (by simp_all)
 
-protected instance Com.decidableEq [DecidableEq Op] [DecidableEq Ty] :
-    {Γ : Ctxt Ty} → {ty : Ty} → DecidableEq (Com Op Γ ty)
+protected instance Com.decidableEq [DecidableEq d.Op] [DecidableEq d.Ty] :
+    {Γ : Ctxt d.Ty} → {ty : d.Ty} → DecidableEq (Com d Γ ty)
   | _, _, .ret v₁, .ret v₂ => decidable_of_iff (v₁ = v₂) (by simp)
   | _, _, .lete (α := α₁) e₁ body₁, .lete (α := α₂) e₂ body₂ =>
     if hα : α₁ = α₂
@@ -120,91 +127,97 @@ protected instance Com.decidableEq [DecidableEq Op] [DecidableEq Ty] :
 
 end
 
-/-- `Lets Op Γ₁ Γ₂` is a sequence of lets which are well-formed under context `Γ₂` and result in
+/-- `Lets d Γ₁ Γ₂` is a sequence of lets which are well-formed under context `Γ₂` and result in
     context `Γ₁`-/
-inductive Lets : Ctxt Ty → Ctxt Ty → Type where
-  | nil {Γ : Ctxt Ty} : Lets Γ Γ
-  | lete (body : Lets Γ₁ Γ₂) (e : Expr Op Γ₂ t) : Lets Γ₁ (Γ₂.snoc t)
-  deriving Repr
+inductive Lets : Ctxt d.Ty → Ctxt d.Ty → Type where
+  | nil {Γ : Ctxt d.Ty} : Lets Γ Γ
+  | lete (body : Lets Γ₁ Γ₂) (e : Expr d Γ₂ t) : Lets Γ₁ (Γ₂.snoc t)
+
+open Std (Format) in
+variable {d} [Repr d.Op] [Repr d.Ty] in
+def Lets.repr (prec : Nat) : Lets d Γ_in Γ_out → Format
+  | .nil => .align false ++ f!"nil"
+  | .lete body e => (.align false ++ f!"{e.repr prec}") ++ body.repr prec
+instance [Repr d.Op] [Repr d.Ty] : Repr (Lets d Γ_in Γ_out) := ⟨flip Lets.repr⟩
 
 /-
   # Definitions
 -/
 
-variable {Op Ty : Type} [OpSignature Op Ty]
+variable {d : Dialect} [OpSignature d]
 
 @[elab_as_elim]
-def Com.rec' {motive : (a : Ctxt Ty) → (a_1 : Ty) → Com Op a a_1 → Sort u} :
-    (ret : {Γ : Ctxt Ty} → {t : Ty} → (v : Var Γ t) → motive Γ t (Com.ret v)) →
-    (lete : {Γ : Ctxt Ty} →
-        {α β : Ty} →
-          (e : Expr Op Γ α) →
-            (body : Com Op (Ctxt.snoc Γ α) β) →
+def Com.rec' {motive : (a : Ctxt d.Ty) → (a_1 : d.Ty) → Com d a a_1 → Sort u} :
+    (ret : {Γ : Ctxt d.Ty} → {t : d.Ty} → (v : Var Γ t) → motive Γ t (Com.ret v)) →
+    (lete : {Γ : Ctxt d.Ty} →
+        {α β : d.Ty} →
+          (e : Expr d Γ α) →
+            (body : Com d (Ctxt.snoc Γ α) β) →
               motive (Ctxt.snoc Γ α) β body → motive Γ β (Com.lete e body)) →
-      {a : Ctxt Ty} → {a_1 : Ty} → (t : Com Op a a_1) → motive a a_1 t
+      {a : Ctxt d.Ty} → {a_1 : d.Ty} → (t : Com d a a_1) → motive a a_1 t
   | hret, _, _, _, Com.ret v => hret v
   | hret, hlete, _, _, Com.lete e body => hlete e body (Com.rec' hret hlete body)
 
-def Expr.op {Γ : Ctxt Ty} {ty : Ty} (e : Expr Op Γ ty) : Op :=
+def Expr.op {Γ : Ctxt d.Ty} {ty : d.Ty} (e : Expr d Γ ty) : d.Op :=
   Expr.casesOn e (fun op _ _ _ => op)
 
-theorem Expr.ty_eq {Γ : Ctxt Ty} {ty : Ty} (e : Expr Op Γ ty) :
+theorem Expr.ty_eq {Γ : Ctxt d.Ty} {ty : d.Ty} (e : Expr d Γ ty) :
     ty = OpSignature.outTy e.op :=
   Expr.casesOn e (fun _ ty_eq _ _ => ty_eq)
 
-def Expr.args {Γ : Ctxt Ty} {ty : Ty} (e : Expr Op Γ ty) :
+def Expr.args {Γ : Ctxt d.Ty} {ty : d.Ty} (e : Expr d Γ ty) :
     HVector (Var Γ) (OpSignature.sig e.op) :=
   Expr.casesOn e (fun _ _ args _ => args)
 
-def Expr.regArgs {Γ : Ctxt Ty} {ty : Ty} (e : Expr Op Γ ty) :
-    HVector (fun t : Ctxt Ty × Ty => Com Op t.1 t.2) (OpSignature.regSig e.op) :=
+def Expr.regArgs {Γ : Ctxt d.Ty} {ty : d.Ty} (e : Expr d Γ ty) :
+    HVector (fun t : Ctxt d.Ty × d.Ty => Com d t.1 t.2) (OpSignature.regSig e.op) :=
   Expr.casesOn e (fun _ _ _ regArgs => regArgs)
 
 /-! Projection equations for `Expr` -/
 @[simp]
-theorem Expr.op_mk {Γ : Ctxt Ty} {ty : Ty} (op : Op) (ty_eq : ty = OpSignature.outTy op)
+theorem Expr.op_mk {Γ : Ctxt d.Ty} {ty : d.Ty} (op : d.Op) (ty_eq : ty = OpSignature.outTy op)
     (args : HVector (Var Γ) (OpSignature.sig op)) (regArgs):
     (Expr.mk op ty_eq args regArgs).op = op := rfl
 
 @[simp]
-theorem Expr.args_mk {Γ : Ctxt Ty} {ty : Ty} (op : Op) (ty_eq : ty = OpSignature.outTy op)
+theorem Expr.args_mk {Γ : Ctxt d.Ty} {ty : d.Ty} (op : d.Op) (ty_eq : ty = OpSignature.outTy op)
     (args : HVector (Var Γ) (OpSignature.sig op)) (regArgs) :
     (Expr.mk op ty_eq args regArgs).args = args := rfl
 
 @[simp]
-theorem Expr.regArgs_mk {Γ : Ctxt Ty} {ty : Ty} (op : Op) (ty_eq : ty = OpSignature.outTy op)
+theorem Expr.regArgs_mk {Γ : Ctxt d.Ty} {ty : d.Ty} (op : d.Op) (ty_eq : ty = OpSignature.outTy op)
     (args : HVector (Var Γ) (OpSignature.sig op)) (regArgs) :
     (Expr.mk op ty_eq args regArgs).regArgs = regArgs := rfl
 
 -- TODO: the following `variable` probably means we include these assumptions also in definitions
 -- that might not strictly need them, we can look into making this more fine-grained
-variable [TyDenote Ty] [OpDenote Op Ty] [DecidableEq Ty]
+variable [TyDenote d.Ty] [OpDenote d] [DecidableEq d.Ty]
 
 mutual
 
-def HVector.denote : {l : List (Ctxt Ty × Ty)} → (T : HVector (fun t => Com Op t.1 t.2) l) →
+def HVector.denote : {l : List (Ctxt d.Ty × d.Ty)} → (T : HVector (fun t => Com d t.1 t.2) l) →
     HVector (fun t => t.1.Valuation → toType t.2) l
   | _, .nil => HVector.nil
   | _, .cons v vs => HVector.cons (v.denote) (HVector.denote vs)
 
-def Expr.denote : {ty : Ty} → (e : Expr Op Γ ty) → (Γv : Valuation Γ) → (toType ty)
+def Expr.denote : {ty : d.Ty} → (e : Expr d Γ ty) → (Γv : Valuation Γ) → (toType ty)
   | _, ⟨op, Eq.refl _, args, regArgs⟩, Γv =>
     OpDenote.denote op (args.map (fun _ v => Γv v)) regArgs.denote
 
-def Com.denote : Com Op Γ ty → (Γv : Valuation Γ) → (toType ty)
+def Com.denote : Com d Γ ty → (Γv : Valuation Γ) → (toType ty)
   | .ret e, Γv => Γv e
   | .lete e body, Γv => body.denote (Γv.snoc (e.denote Γv))
 
 end
 
 @[simp]
-theorem Com.denote_lete (e : Expr Op Γ α) (body : Com Op (Γ.snoc α) β) :
+theorem Com.denote_lete (e : Expr d Γ α) (body : Com d (Γ.snoc α) β) :
   Com.denote (Com.lete e body) = fun Γv => body.denote (Γv.snoc (e.denote Γv)) := by
     funext Γv; simp[Com.denote]
 
 @[simp]
 theorem Com.denote_ret (v : Var Γ α)  :
-  Com.denote (Op := Op) (Com.ret v) = fun Γv => Γv v := by
+  Com.denote (d:=d) (Com.ret v) = fun Γv => Γv v := by
     funext Γv; simp[Com.denote]
 
 /-
@@ -223,7 +236,7 @@ args, since there now are equation lemmas for it.
 #eval Lean.Meta.getEqnsFor? ``Expr.denote
 #eval Lean.Meta.getEqnsFor? ``Com.denote
 
-def Lets.denote : Lets Op Γ₁ Γ₂ → Valuation Γ₁ → Valuation Γ₂
+def Lets.denote : Lets d Γ₁ Γ₂ → Valuation Γ₁ → Valuation Γ₂
   | .nil => id
   | .lete e body => fun ll t v => by
     cases v using Var.casesOn with
@@ -235,13 +248,13 @@ def Lets.denote : Lets Op Γ₁ Γ₂ → Valuation Γ₁ → Valuation Γ₂
       exact e.denote ll v
 
 def Expr.changeVars (varsMap : Γ.Hom Γ') :
-    {ty : Ty} → (e : Expr Op Γ ty) → Expr Op Γ' ty
+    {ty : d.Ty} → (e : Expr d Γ ty) → Expr d Γ' ty
   | _, ⟨op, Eq.refl _, args, regArgs⟩ => ⟨op, rfl, args.map varsMap, regArgs⟩
 
 @[simp]
-theorem Expr.denote_changeVars {Γ Γ' : Ctxt Ty}
+theorem Expr.denote_changeVars {Γ Γ' : Ctxt d.Ty}
     (varsMap : Γ.Hom Γ')
-    (e : Expr Op Γ ty)
+    (e : Expr d Γ ty)
     (Γ'v : Valuation Γ') :
     (e.changeVars varsMap).denote Γ'v =
     e.denote (fun t v => Γ'v (varsMap v)) := by
@@ -250,14 +263,14 @@ theorem Expr.denote_changeVars {Γ Γ' : Ctxt Ty}
 
 def Com.changeVars
     (varsMap : Γ.Hom Γ') :
-    Com Op Γ ty → Com Op Γ' ty
+    Com d Γ ty → Com d Γ' ty
   | .ret e => .ret (varsMap e)
   | .lete e body => .lete (e.changeVars varsMap)
       (body.changeVars (fun t v => varsMap.snocMap v))
 
 @[simp]
 theorem Com.denote_changeVars
-    (varsMap : Γ.Hom Γ') (c : Com Op Γ ty)
+    (varsMap : Γ.Hom Γ') (c : Com d Γ ty)
     (Γ'v : Valuation Γ') :
     (c.changeVars varsMap).denote Γ'v =
     c.denote (fun t v => Γ'v (varsMap v)) := by
@@ -271,13 +284,13 @@ theorem Com.denote_changeVars
     cases v using Var.casesOn <;> simp
 
 
-variable (Op : _) {Ty : _} [OpSignature Op Ty] in
+variable (d : Dialect) [OpSignature d] in
 /-- The result returned by `addProgramToLets` -/
-structure addProgramToLets.Result (Γ_in Γ_out : Ctxt Ty) (ty : Ty) where
+structure addProgramToLets.Result (Γ_in Γ_out : Ctxt d.Ty) (ty : d.Ty) where
   /-- The new out context -/
-  {Γ_out_new : Ctxt Ty}
+  {Γ_out_new : Ctxt d.Ty}
   /-- The new `lets`, with the program added to it -/
-  lets : Lets Op Γ_in Γ_out_new
+  lets : Lets d Γ_in Γ_out_new
   /-- The difference between the old out context and the new out context
       This induces a context mapping from `Γ_out` to `Γ_out_new` -/
   diff : Ctxt.Diff Γ_out Γ_out_new
@@ -291,15 +304,15 @@ structure addProgramToLets.Result (Γ_in Γ_out : Ctxt Ty) (ty : Ty) where
   * a variable in the new out context, which is semantically equivalent to the return variable of
     the added program
 -/
-def addProgramToLets (lets : Lets Op Γ_in Γ_out) (varsMap : Δ.Hom Γ_out) : Com Op Δ ty →
-    addProgramToLets.Result Op Γ_in Γ_out ty
+def addProgramToLets (lets : Lets d Γ_in Γ_out) (varsMap : Δ.Hom Γ_out) : Com d Δ ty →
+    addProgramToLets.Result d Γ_in Γ_out ty
   | .ret v => ⟨lets, .zero _, varsMap v⟩
   | .lete (α:=α) e body =>
       let lets := Lets.lete lets (e.changeVars varsMap)
       let ⟨lets', diff, v'⟩ := addProgramToLets lets (varsMap.snocMap) body
       ⟨lets', diff.unSnoc, v'⟩
 
-theorem denote_addProgramToLets_lets (lets : Lets Op Γ_in Γ_out) {map} {com : Com Op Δ t}
+theorem denote_addProgramToLets_lets (lets : Lets d Γ_in Γ_out) {map} {com : Com d Δ t}
     (ll : Valuation Γ_in) ⦃t⦄ (var : Var Γ_out t) :
     (addProgramToLets lets map com).lets.denote ll ((addProgramToLets lets map com).diff.toHom var)
     = lets.denote ll var := by
@@ -311,7 +324,7 @@ theorem denote_addProgramToLets_lets (lets : Lets Op Γ_in Γ_out) {map} {com : 
     rw [addProgramToLets]
     simp [ih, Lets.denote]
 
-theorem denote_addProgramToLets_var {lets : Lets Op Γ_in Γ_out} {map} {com : Com Op Δ t} :
+theorem denote_addProgramToLets_var {lets : Lets d Γ_in Γ_out} {map} {com : Com d Δ t} :
     ∀ (ll : Valuation Γ_in),
       (addProgramToLets lets map com).lets.denote ll (addProgramToLets lets map com).var
       = com.denote (fun _ v => lets.denote ll <| map v) := by
@@ -330,13 +343,13 @@ theorem denote_addProgramToLets_var {lets : Lets Op Γ_in Γ_out} {map} {com : C
     . simp [Lets.denote]; rfl
 
 /-- Add some `Lets` to the beginning of a program -/
-def addLetsAtTop : (lets : Lets Op Γ₁ Γ₂) → (inputProg : Com Op Γ₂ t₂) → Com Op Γ₁ t₂
+def addLetsAtTop : (lets : Lets d Γ₁ Γ₂) → (inputProg : Com d Γ₂ t₂) → Com d Γ₁ t₂
   | Lets.nil, inputProg => inputProg
   | Lets.lete body e, inputProg =>
     addLetsAtTop body (.lete e inputProg)
 
 theorem denote_addLetsAtTop :
-    (lets : Lets Op Γ₁ Γ₂) → (inputProg : Com Op Γ₂ t₂) →
+    (lets : Lets d Γ₁ Γ₂) → (inputProg : Com d Γ₂ t₂) →
     (addLetsAtTop lets inputProg).denote =
       inputProg.denote ∘ lets.denote
   | Lets.nil, inputProg => rfl
@@ -353,18 +366,18 @@ theorem denote_addLetsAtTop :
 `lets`, `rhs` and `inputProg`, while reassigning `v`, a free variable in
 `inputProg`, to the output of `rhs`. It also assigns all free variables
 in `rhs` to variables available at the end of `lets` using `map`. -/
-def addProgramInMiddle {Γ₁ Γ₂ Γ₃ : Ctxt Ty} (v : Var Γ₂ t₁)
+def addProgramInMiddle {Γ₁ Γ₂ Γ₃ : Ctxt d.Ty} (v : Var Γ₂ t₁)
     (map : Γ₃.Hom Γ₂)
-    (lets : Lets Op Γ₁ Γ₂) (rhs : Com Op Γ₃ t₁)
-    (inputProg : Com Op Γ₂ t₂) : Com Op Γ₁ t₂ :=
+    (lets : Lets d Γ₁ Γ₂) (rhs : Com d Γ₃ t₁)
+    (inputProg : Com d Γ₂ t₂) : Com d Γ₁ t₂ :=
   let r := addProgramToLets lets map rhs
   addLetsAtTop r.lets <| inputProg.changeVars (r.diff.toHom.with v r.var)
 
-theorem denote_addProgramInMiddle {Γ₁ Γ₂ Γ₃ : Ctxt Ty}
+theorem denote_addProgramInMiddle {Γ₁ Γ₂ Γ₃ : Ctxt d.Ty}
     (v : Var Γ₂ t₁) (s : Valuation Γ₁)
     (map : Γ₃.Hom Γ₂)
-    (lets : Lets Op Γ₁ Γ₂) (rhs : Com Op Γ₃ t₁)
-    (inputProg : Com Op Γ₂ t₂) :
+    (lets : Lets d Γ₁ Γ₂) (rhs : Com d Γ₃ t₁)
+    (inputProg : Com d Γ₂ t₂) :
     (addProgramInMiddle v map lets rhs inputProg).denote s =
       inputProg.denote (fun t' v' =>
         let s' := lets.denote s
@@ -388,22 +401,22 @@ theorem denote_addProgramInMiddle {Γ₁ Γ₂ Γ₃ : Ctxt Ty}
   next =>
     apply denote_addProgramToLets_lets
 
-structure FlatCom (Op : _) {Ty : _} [OpSignature Op Ty] (Γ : Ctxt Ty) (t : Ty) where
-  {Γ_out : Ctxt Ty}
+structure FlatCom (d : Dialect) [OpSignature d] (Γ : Ctxt d.Ty) (t : d.Ty) where
+  {Γ_out : Ctxt d.Ty}
   /-- The let bindings of the original program -/
-  lets : Lets Op Γ Γ_out
+  lets : Lets d Γ Γ_out
   /-- The return variable -/
   ret : Var Γ_out t
 
-def Com.toLets {t : Ty} : Com Op Γ t → FlatCom Op Γ t :=
+def Com.toLets {t : d.Ty} : Com d Γ t → FlatCom d Γ t :=
   go .nil
 where
-  go {Γ_out} (lets : Lets Op Γ Γ_out) : Com Op Γ_out t → FlatCom Op Γ t
+  go {Γ_out} (lets : Lets d Γ Γ_out) : Com d Γ_out t → FlatCom d Γ t
     | .ret v => ⟨lets, v⟩
     | .lete e body => go (lets.lete e) body
 
 @[simp]
-theorem Com.denote_toLets_go (lets : Lets Op Γ_in Γ_out) (com : Com Op Γ_out t) (s : Valuation Γ_in) :
+theorem Com.denote_toLets_go (lets : Lets d Γ_in Γ_out) (com : Com d Γ_out t) (s : Valuation Γ_in) :
     (toLets.go lets com).lets.denote s (toLets.go lets com).ret = com.denote (lets.denote s) := by
   induction com using Com.rec'
   . rfl
@@ -416,15 +429,15 @@ theorem Com.denote_toLets_go (lets : Lets Op Γ_in Γ_out) (com : Com Op Γ_out 
     cases v using Var.casesOn <;> simp[Lets.denote]
 
 @[simp]
-theorem Com.denote_toLets (com : Com Op Γ t) (s : Valuation Γ) :
+theorem Com.denote_toLets (com : Com d Γ t) (s : Valuation Γ) :
     com.toLets.lets.denote s com.toLets.ret = com.denote s :=
   denote_toLets_go ..
 
 /-- Get the `Expr` that a var `v` is assigned to in a sequence of `Lets`,
     without adjusting variables
 -/
-def Lets.getExprAux {Γ₁ Γ₂ : Ctxt Ty} {t : Ty} : Lets Op Γ₁ Γ₂ → Var Γ₂ t →
-    Option ((Δ : Ctxt Ty) × Expr Op Δ t)
+def Lets.getExprAux {Γ₁ Γ₂ : Ctxt d.Ty} {t : d.Ty} : Lets d Γ₁ Γ₂ → Var Γ₂ t →
+    Option ((Δ : Ctxt d.Ty) × Expr d Δ t)
   | .nil, _ => none
   | .lete lets e, v => by
     cases v using Var.casesOn with
@@ -435,7 +448,7 @@ def Lets.getExprAux {Γ₁ Γ₂ : Ctxt Ty} {t : Ty} : Lets Op Γ₁ Γ₂ → V
     then the orignal context `Γ₁` is a prefix of the local context `Δ`, and
     their difference is exactly the value of the requested variable index plus 1
 -/
-def Lets.getExprAuxDiff {lets : Lets Op Γ₁ Γ₂} {v : Var Γ₂ t}
+def Lets.getExprAuxDiff {lets : Lets d Γ₁ Γ₂} {v : Var Γ₂ t}
     (h : getExprAux lets v = some ⟨Δ, e⟩) :
     Δ.Diff Γ₂ :=
   ⟨v.val + 1, by
@@ -455,8 +468,8 @@ def Lets.getExprAuxDiff {lets : Lets Op Γ₁ Γ₂} {v : Var Γ₂ t}
         exact a
   ⟩
 
-theorem Lets.denote_getExprAux {Γ₁ Γ₂ Δ : Ctxt Ty} {t : Ty}
-    {lets : Lets Op Γ₁ Γ₂} {v : Var Γ₂ t} {e : Expr Op Δ t}
+theorem Lets.denote_getExprAux {Γ₁ Γ₂ Δ : Ctxt d.Ty} {t : d.Ty}
+    {lets : Lets d Γ₁ Γ₂} {v : Var Γ₂ t} {e : Expr d Δ t}
     (he : lets.getExprAux v = some ⟨Δ, e⟩)
     (s : Valuation Γ₁) :
     (e.changeVars (getExprAuxDiff he).toHom).denote (lets.denote s) = (lets.denote s) v := by
@@ -480,14 +493,14 @@ theorem Lets.denote_getExprAux {Γ₁ Γ₂ Δ : Ctxt Ty} {t : Ty}
 /-- Get the `Expr` that a var `v` is assigned to in a sequence of `Lets`.
 The variables are adjusted so that they are variables in the output context of a lets,
 not the local context where the variable appears. -/
-def Lets.getExpr {Γ₁ Γ₂ : Ctxt Ty} (lets : Lets Op Γ₁ Γ₂) {t : Ty} (v : Var Γ₂ t) :
-    Option (Expr Op Γ₂ t) :=
+def Lets.getExpr {Γ₁ Γ₂ : Ctxt d.Ty} (lets : Lets d Γ₁ Γ₂) {t : d.Ty} (v : Var Γ₂ t) :
+    Option (Expr d Γ₂ t) :=
   match h : getExprAux lets v with
   | none => none
   | some r => r.snd.changeVars (getExprAuxDiff h).toHom
 
-theorem Lets.denote_getExpr {Γ₁ Γ₂ : Ctxt Ty} : {lets : Lets Op Γ₁ Γ₂} → {t : Ty} →
-    {v : Var Γ₂ t} → {e : Expr Op Γ₂ t} → (he : lets.getExpr v = some e) → (s : Valuation Γ₁) →
+theorem Lets.denote_getExpr {Γ₁ Γ₂ : Ctxt d.Ty} : {lets : Lets d Γ₁ Γ₂} → {t : d.Ty} →
+    {v : Var Γ₂ t} → {e : Expr d Γ₂ t} → (he : lets.getExpr v = some e) → (s : Valuation Γ₁) →
     e.denote (lets.denote s) = (lets.denote s) v := by
   intros lets _ v e he s
   simp [getExpr] at he
@@ -513,34 +526,33 @@ instance : Functor Signature where
 /-- A dialect morphism consists of a map between operations and a map between types,
   such that the signature of operations is respected
 -/
-structure DialectMorphism (Op Op' : Type) {Ty Ty' : Type} [OpSignature Op Ty] [OpSignature Op' Ty'] where
-  mapOp : Op → Op'
-  mapTy : Ty → Ty'
+structure DialectMorphism (d d' : Dialect) [OpSignature d] [OpSignature d'] where
+  mapOp : d.Op → d'.Op
+  mapTy : d.Ty → d'.Ty
   preserves_signature : ∀ op, signature (mapOp op) = mapTy <$> (signature op)
 
-variable {Op Op' Ty Ty : Type} [OpSignature Op Ty] [OpSignature Op' Ty']
-  (f : DialectMorphism Op Op')
+variable {d d'} [OpSignature d] [OpSignature d'] (f : DialectMorphism d d')
 
-def DialectMorphism.preserves_sig (op : Op) :
+def DialectMorphism.preserves_sig (op : d.Op) :
     OpSignature.sig (f.mapOp op) = f.mapTy <$> (OpSignature.sig op) := by
   simp only [OpSignature.sig, Function.comp_apply, f.preserves_signature, List.map_eq_map]; rfl
 
-def DialectMorphism.preserves_regSig (op : Op) :
+def DialectMorphism.preserves_regSig (op : d.Op) :
     OpSignature.regSig (f.mapOp op) = (OpSignature.regSig op).map (
       fun ⟨a, b⟩ => ⟨f.mapTy <$> a, f.mapTy b⟩
     ) := by
   simp only [OpSignature.regSig, Function.comp_apply, f.preserves_signature, List.map_eq_map]; rfl
 
-def DialectMorphism.preserves_outTy (op : Op) :
+def DialectMorphism.preserves_outTy (op : d.Op) :
     OpSignature.outTy (f.mapOp op) = f.mapTy (OpSignature.outTy op) := by
   simp only [OpSignature.outTy, Function.comp_apply, f.preserves_signature]; rfl
 
 mutual
-  def Com.map : Com Op Γ ty → Com Op' (f.mapTy <$> Γ) (f.mapTy ty)
+  def Com.map : Com d Γ ty → Com d' (f.mapTy <$> Γ) (f.mapTy ty)
     | .ret v          => .ret v.toMap
     | .lete body rest => .lete body.map rest.map
 
-  def Expr.map : Expr Op (Ty:=Ty) Γ ty → Expr Op' (Ty:=Ty') (Γ.map f.mapTy) (f.mapTy ty)
+  def Expr.map : Expr d Γ ty → Expr d' (Γ.map f.mapTy) (f.mapTy ty)
     | ⟨op, Eq.refl _, args, regs⟩ => ⟨
         f.mapOp op,
         (f.preserves_outTy _).symm,
@@ -550,9 +562,9 @@ mutual
       ⟩
 
   /-- Inline of `HVector.map'` for the termination checker -/
-  def HVector.mapDialectMorphism : ∀ {regSig : RegionSignature Ty},
-      HVector (fun t => Com Op t.fst t.snd) regSig
-      → HVector (fun t => Com Op' t.fst t.snd) (f.mapTy <$> regSig : RegionSignature _)
+  def HVector.mapDialectMorphism : ∀ {regSig : RegionSignature d.Ty},
+      HVector (fun t => Com d t.fst t.snd) regSig
+      → HVector (fun t => Com d' t.fst t.snd) (f.mapTy <$> regSig : RegionSignature _)
     | _, .nil        => .nil
     | t::_, .cons a as  => .cons a.map (HVector.mapDialectMorphism as)
 end
@@ -563,24 +575,24 @@ end Map
   ## Matching
 -/
 
-abbrev Mapping (Γ Δ : Ctxt Ty) : Type :=
+abbrev Mapping (Γ Δ : Ctxt d.Ty) : Type :=
   @AList (Σ t, Var Γ t) (fun x => Var Δ x.1)
 
-def HVector.toVarSet : {l : List Ty} → (T : HVector (Var Γ) l) → VarSet Γ
+def HVector.toVarSet : {l : List d.Ty} → (T : HVector (Var Γ) l) → VarSet Γ
   | [], .nil => ∅
   | _::_, .cons v vs => insert ⟨_, v⟩ vs.toVarSet
 
-def HVector.vars {l : List Ty}
+def HVector.vars {l : List d.Ty}
     (T : HVector (Var Γ) l) : VarSet Γ :=
   T.foldl (fun _ s a => insert ⟨_, a⟩ s) ∅
 
 @[simp]
 theorem HVector.vars_nil :
-    (HVector.nil : HVector (Var Γ) ([] : List Ty)).vars = ∅ := by
+    (HVector.nil : HVector (Var Γ) ([] : List d.Ty)).vars = ∅ := by
   simp [HVector.vars, HVector.foldl]
 
 @[simp]
-theorem HVector.vars_cons {t  : Ty} {l : List Ty}
+theorem HVector.vars_cons {t  : d.Ty} {l : List d.Ty}
     (v : Var Γ t) (T : HVector (Var Γ) l) :
     (HVector.cons v T).vars = insert ⟨_, v⟩ T.vars := by
   rw [HVector.vars, HVector.vars]
@@ -597,7 +609,7 @@ theorem HVector.vars_cons {t  : Ty} {l : List Ty}
     simp [Finset.ext_iff, or_comm, or_assoc]
 
 /-- The free variables of `lets` that are (transitively) referred to by some variable `v` -/
-def Lets.vars : Lets Op Γ_in Γ_out → Var Γ_out t → VarSet Γ_in
+def Lets.vars : Lets d Γ_in Γ_out → Var Γ_out t → VarSet Γ_in
   | .nil, v => VarSet.ofVar v
   | .lete lets e, v => by
       cases v using Var.casesOn with
@@ -605,7 +617,7 @@ def Lets.vars : Lets Op Γ_in Γ_out → Var Γ_out t → VarSet Γ_in
       -- this is wrong
       | last => exact (e.args.vars).biUnion (fun v => lets.vars v.2)
 
-theorem HVector.map_eq_of_eq_on_vars {A : Ty → Type*}
+theorem HVector.map_eq_of_eq_on_vars {A : d.Ty → Type*}
     {T : HVector (Var Γ) l}
     {s₁ s₂ : ∀ (t), Var Γ t → A t}
     (h : ∀ v, v ∈ T.vars → s₁ _ v.2 = s₂ _ v.2) :
@@ -621,7 +633,7 @@ theorem HVector.map_eq_of_eq_on_vars {A : Ty → Type*}
       apply h
       simp_all
 
-theorem Lets.denote_eq_of_eq_on_vars (lets : Lets Op Γ_in Γ_out)
+theorem Lets.denote_eq_of_eq_on_vars (lets : Lets d Γ_in Γ_out)
     (v : Var Γ_out t)
     {s₁ s₂ : Valuation Γ_in}
     (h : ∀ w, w ∈ lets.vars v → s₁ w.2 = s₂ w.2) :
@@ -648,7 +660,7 @@ theorem Lets.denote_eq_of_eq_on_vars (lets : Lets Op Γ_in Γ_out)
       simp
       use v.1, v.2
 
-def Com.vars : Com Op Γ t → VarSet Γ :=
+def Com.vars : Com d Γ t → VarSet Γ :=
   fun com => com.toLets.lets.vars com.toLets.ret
 
 /--
@@ -659,23 +671,23 @@ def Com.vars : Com Op Γ t → VarSet Γ :=
   If this succeeds, return the mapping.
 -/
 
-def matchVar {Γ_in Γ_out Δ_in Δ_out : Ctxt Ty} {t : Ty} [DecidableEq Op]
-    (lets : Lets Op Γ_in Γ_out) (v : Var Γ_out t) :
-    (matchLets : Lets Op Δ_in Δ_out) →
+def matchVar {Γ_in Γ_out Δ_in Δ_out : Ctxt d.Ty} {t : d.Ty} [DecidableEq d.Op]
+    (lets : Lets d Γ_in Γ_out) (v : Var Γ_out t) :
+    (matchLets : Lets d Δ_in Δ_out) →
     (w : Var Δ_out t) →
     (ma : Mapping Δ_in Γ_out := ∅) →
     Option (Mapping Δ_in Γ_out)
   | .lete matchLets _, ⟨w+1, h⟩, ma => -- w† = Var.toSnoc w
       let w := ⟨w, by simp_all[Ctxt.snoc]⟩
       matchVar lets v matchLets w ma
-  | @Lets.lete _ _ _ _ Δ_out _ matchLets matchExpr, ⟨0, _⟩, ma => do -- w† = Var.last
+  | @Lets.lete _ _ _ Δ_out _ matchLets matchExpr, ⟨0, _⟩, ma => do -- w† = Var.last
       let ie ← lets.getExpr v
       if hs : ∃ h : ie.op = matchExpr.op, ie.regArgs = (h ▸ matchExpr.regArgs)
       then
         -- hack to make a termination proof work
         let matchVar' := fun t vₗ vᵣ ma =>
             matchVar (t := t) lets vₗ matchLets vᵣ ma
-        let rec matchArg : ∀ {l : List Ty}
+        let rec matchArg : ∀ {l : List d.Ty}
             (_Tₗ : HVector (Var Γ_out) l) (_Tᵣ :  HVector (Var Δ_out) l),
             Mapping Δ_in Γ_out → Option (Mapping Δ_in Γ_out)
           | _, .nil, .nil, ma => some ma
@@ -696,13 +708,13 @@ def matchVar {Γ_in Γ_out Δ_in Δ_out : Ctxt Ty} {t : Ty} [DecidableEq Op]
 open AList
 
 theorem subset_entries_matchVar_matchArg_aux
-    {Γ_out Δ_in Δ_out  : Ctxt Ty}
-    {matchVar' : (t : Ty) → Var Γ_out t → Var Δ_out t →
+    {Γ_out Δ_in Δ_out  : Ctxt d.Ty}
+    {matchVar' : (t : d.Ty) → Var Γ_out t → Var Δ_out t →
       Mapping Δ_in Γ_out → Option (Mapping Δ_in Γ_out)} :
-    {l : List Ty} → {argsₗ : HVector (Var Γ_out) l} →
+    {l : List d.Ty} → {argsₗ : HVector (Var Γ_out) l} →
     {argsᵣ : HVector (Var Δ_out) l} → {ma : Mapping Δ_in Γ_out} →
     {varMap : Mapping Δ_in Γ_out} →
-    (hmatchVar : ∀ vMap (t : Ty) (vₗ vᵣ) ma,
+    (hmatchVar : ∀ vMap (t : d.Ty) (vₗ vᵣ) ma,
         vMap ∈ matchVar' t vₗ vᵣ ma → ma.entries ⊆ vMap.entries) →
     (hvarMap : varMap ∈ matchVar.matchArg Δ_out matchVar' argsₗ argsᵣ ma) →
     ma.entries ⊆ varMap.entries
@@ -718,10 +730,10 @@ theorem subset_entries_matchVar_matchArg_aux
     exact hmatchVar _ _ _ _ _ h₁
 
 /-- The output mapping of `matchVar` extends the input mapping when it succeeds. -/
-theorem subset_entries_matchVar [DecidableEq Op]
+theorem subset_entries_matchVar [DecidableEq d.Op]
     {varMap : Mapping Δ_in Γ_out} {ma : Mapping Δ_in Γ_out}
-    {lets : Lets Op Γ_in Γ_out} {v : Var Γ_out t} :
-    {matchLets : Lets Op Δ_in Δ_out} → {w : Var Δ_out t} →
+    {lets : Lets d Γ_in Γ_out} {v : Var Γ_out t} :
+    {matchLets : Lets d Δ_in Δ_out} → {w : Var Δ_out t} →
     (hvarMap : varMap ∈ matchVar lets v matchLets w ma) →
     ma.entries ⊆ varMap.entries
   | .nil, w => by
@@ -756,10 +768,10 @@ theorem subset_entries_matchVar [DecidableEq Op]
         exact subset_entries_matchVar_matchArg_aux
           (fun vMap t vₗ vᵣ ma hvMap => subset_entries_matchVar hvMap) h
 
-theorem subset_entries_matchVar_matchArg [DecidableEq Op]
-    {Γ_in Γ_out Δ_in Δ_out : Ctxt Ty} {lets : Lets Op Γ_in Γ_out}
-    {matchLets : Lets Op Δ_in Δ_out} :
-    {l : List Ty} → {argsₗ : HVector (Var Γ_out) l} →
+theorem subset_entries_matchVar_matchArg [DecidableEq d.Op]
+    {Γ_in Γ_out Δ_in Δ_out : Ctxt d.Ty} {lets : Lets d Γ_in Γ_out}
+    {matchLets : Lets d Δ_in Δ_out} :
+    {l : List d.Ty} → {argsₗ : HVector (Var Γ_out) l} →
     {argsᵣ : HVector (Var Δ_out) l} → {ma : Mapping Δ_in Γ_out} →
     {varMap : Mapping Δ_in Γ_out} →
     (hvarMap : varMap ∈ matchVar.matchArg Δ_out
@@ -769,22 +781,22 @@ theorem subset_entries_matchVar_matchArg [DecidableEq Op]
   subset_entries_matchVar_matchArg_aux (fun _ _ _ _ _ => subset_entries_matchVar)
 
 -- TODO: this assumption is too strong, we also want to be able to model non-inhabited types
-variable [∀ (t : Ty), Inhabited (toType t)] [DecidableEq Op]
+variable [∀ (t : d.Ty), Inhabited (toType t)] [DecidableEq d.Op]
 
-theorem denote_matchVar_matchArg [DecidableEq Op]
-    {Γ_out Δ_in Δ_out : Ctxt Ty} {lets : Lets Op Γ_in Γ_out}
-    {matchLets : Lets Op Δ_in Δ_out} :
-    {l : List Ty} →
+theorem denote_matchVar_matchArg [DecidableEq d.Op]
+    {Γ_out Δ_in Δ_out : Ctxt d.Ty} {lets : Lets d Γ_in Γ_out}
+    {matchLets : Lets d Δ_in Δ_out} :
+    {l : List d.Ty} →
     {args₁ : HVector (Var Γ_out) l} →
     {args₂ : HVector (Var Δ_out) l} →
     {ma varMap₁ varMap₂ : Mapping Δ_in Γ_out} →
     (h_sub : varMap₁.entries ⊆ varMap₂.entries) →
-    (f₁ : (t : Ty) → Var Γ_out t → toType t) →
-    (f₂ : (t : Ty) → Var Δ_out t → toType t) →
+    (f₁ : (t : d.Ty) → Var Γ_out t → toType t) →
+    (f₂ : (t : d.Ty) → Var Δ_out t → toType t) →
     (hf : ∀ t v₁ v₂ (ma : Mapping Δ_in Γ_out) (ma'),
       (ma ∈ matchVar lets v₁ matchLets v₂ ma') →
       ma.entries ⊆ varMap₂.entries → f₂ t v₂ = f₁ t v₁) →
-    (hmatchVar : ∀ vMap (t : Ty) (vₗ vᵣ) ma,
+    (hmatchVar : ∀ vMap (t : d.Ty) (vₗ vᵣ) ma,
       vMap ∈ matchVar (t := t) lets vₗ matchLets vᵣ ma →
       ma.entries ⊆ vMap.entries) →
     (hvarMap : varMap₁ ∈ matchVar.matchArg Δ_out
@@ -806,11 +818,11 @@ theorem denote_matchVar_matchArg [DecidableEq Op]
     · exact hmatchVar
 
 theorem denote_matchVar_of_subset
-    {lets : Lets Op Γ_in Γ_out} {v : Var Γ_out t}
+    {lets : Lets d Γ_in Γ_out} {v : Var Γ_out t}
     {varMap₁ varMap₂ : Mapping Δ_in Γ_out}
     {s₁ : Valuation Γ_in}
     {ma : Mapping Δ_in Γ_out} :
-    {matchLets : Lets Op Δ_in Δ_out} → {w : Var Δ_out t} →
+    {matchLets : Lets d Δ_in Δ_out} → {w : Var Δ_out t} →
     (h_sub : varMap₁.entries ⊆ varMap₂.entries) →
     (h_matchVar : varMap₁ ∈ matchVar lets v matchLets w ma) →
       matchLets.denote (fun t' v' => by
@@ -870,10 +882,10 @@ theorem denote_matchVar_of_subset
           subst hop
           rfl
 
-theorem denote_matchVar {lets : Lets Op Γ_in Γ_out} {v : Var Γ_out t} {varMap : Mapping Δ_in Γ_out}
+theorem denote_matchVar {lets : Lets d Γ_in Γ_out} {v : Var Γ_out t} {varMap : Mapping Δ_in Γ_out}
     {s₁ : Valuation Γ_in}
     {ma : Mapping Δ_in Γ_out}
-    {matchLets : Lets Op Δ_in Δ_out}
+    {matchLets : Lets d Δ_in Δ_out}
     {w : Var Δ_out t} :
     varMap ∈ matchVar lets v matchLets w ma →
     matchLets.denote (fun t' v' => by
@@ -897,9 +909,9 @@ macro_rules | `(tactic| decreasing_trivial) => `(tactic| simp (config := {arith 
 mutual
 
 theorem mem_matchVar_matchArg
-    {Γ_in Γ_out Δ_in Δ_out : Ctxt Ty} {lets : Lets Op Γ_in Γ_out}
-    {matchLets : Lets Op Δ_in Δ_out} :
-    {l : List Ty} → {argsₗ : HVector (Var Γ_out) l} →
+    {Γ_in Γ_out Δ_in Δ_out : Ctxt d.Ty} {lets : Lets d Γ_in Γ_out}
+    {matchLets : Lets d Δ_in Δ_out} :
+    {l : List d.Ty} → {argsₗ : HVector (Var Γ_out) l} →
     {argsᵣ : HVector (Var Δ_out) l} → {ma : Mapping Δ_in Γ_out} →
     {varMap : Mapping Δ_in Γ_out} →
     (hvarMap : varMap ∈ matchVar.matchArg Δ_out
@@ -923,8 +935,8 @@ theorem mem_matchVar_matchArg
 /-- All variables containing in `matchExpr` are assigned by `matchVar`. -/
 theorem mem_matchVar
     {varMap : Mapping Δ_in Γ_out} {ma : Mapping Δ_in Γ_out}
-    {lets : Lets Op Γ_in Γ_out} {v : Var Γ_out t} :
-    {matchLets : Lets Op Δ_in Δ_out} → {w : Var Δ_out t} →
+    {lets : Lets d Γ_in Γ_out} {v : Var Γ_out t} :
+    {matchLets : Lets d Δ_in Δ_out} → {w : Var Δ_out t} →
     (hvarMap : varMap ∈ matchVar lets v matchLets w ma) →
     ∀ {t' v'}, ⟨t', v'⟩ ∈ matchLets.vars w → ⟨t', v'⟩ ∈ varMap
   | .nil, w, h, t', v' => by
@@ -972,8 +984,8 @@ end
 
 /-- A version of `matchVar` that returns a `Hom` of `Ctxt`s instead of the `AList`,
 provided every variable in the context appears as a free variable in `matchExpr`. -/
-def matchVarMap {Γ_in Γ_out Δ_in Δ_out : Ctxt Ty} {t : Ty}
-    (lets : Lets Op Γ_in Γ_out) (v : Var Γ_out t) (matchLets : Lets Op Δ_in Δ_out) (w : Var Δ_out t)
+def matchVarMap {Γ_in Γ_out Δ_in Δ_out : Ctxt d.Ty} {t : d.Ty}
+    (lets : Lets d Γ_in Γ_out) (v : Var Γ_out t) (matchLets : Lets d Δ_in Δ_out) (w : Var Δ_out t)
     (hvars : ∀ t (v : Var Δ_in t), ⟨t, v⟩ ∈ matchLets.vars w) :
     Option (Δ_in.Hom Γ_out) := do
   match hm : matchVar lets v matchLets w with
@@ -986,10 +998,10 @@ def matchVarMap {Γ_in Γ_out Δ_in Δ_out : Ctxt Ty} {t : Ty}
       have := AList.lookup_isSome.2 (mem_matchVar hm (hvars t v'))
       simp_all
 
-theorem denote_matchVarMap {Γ_in Γ_out Δ_in Δ_out : Ctxt Ty}
-    {lets : Lets Op Γ_in Γ_out}
-    {t : Ty} {v : Var Γ_out t}
-    {matchLets : Lets Op Δ_in Δ_out}
+theorem denote_matchVarMap {Γ_in Γ_out Δ_in Δ_out : Ctxt d.Ty}
+    {lets : Lets d Γ_in Γ_out}
+    {t : d.Ty} {v : Var Γ_out t}
+    {matchLets : Lets d Δ_in Δ_out}
     {w : Var Δ_out t}
     {hvars : ∀ t (v : Var Δ_in t), ⟨t, v⟩ ∈ matchLets.vars w}
     {map : Δ_in.Hom Γ_out}
@@ -1016,17 +1028,17 @@ theorem denote_matchVarMap {Γ_in Γ_out Δ_in Δ_out : Ctxt Ty}
 with the `pos`th variable in `prog`, and an `Com` starting with the next variable.
 It also returns, the type of this variable and the variable itself as an element
 of the output `Ctxt` of the returned `Lets`.  -/
-def splitProgramAtAux : (pos : ℕ) → (lets : Lets Op Γ₁ Γ₂) →
-    (prog : Com Op Γ₂ t) →
-    Option (Σ (Γ₃ : Ctxt Ty), Lets Op Γ₁ Γ₃ × Com Op Γ₃ t × (t' : Ty) × Var Γ₃ t')
+def splitProgramAtAux : (pos : ℕ) → (lets : Lets d Γ₁ Γ₂) →
+    (prog : Com d Γ₂ t) →
+    Option (Σ (Γ₃ : Ctxt d.Ty), Lets d Γ₁ Γ₃ × Com d Γ₃ t × (t' : d.Ty) × Var Γ₃ t')
   | 0, lets, .lete e body => some ⟨_, .lete lets e, body, _, Var.last _ _⟩
   | _, _, .ret _ => none
   | n+1, lets, .lete e body =>
     splitProgramAtAux n (lets.lete e) body
 
-theorem denote_splitProgramAtAux : {pos : ℕ} → {lets : Lets Op Γ₁ Γ₂} →
-    {prog : Com Op Γ₂ t} →
-    {res : Σ (Γ₃ : Ctxt Ty), Lets Op Γ₁ Γ₃ × Com Op Γ₃ t × (t' : Ty) × Var Γ₃ t'} →
+theorem denote_splitProgramAtAux : {pos : ℕ} → {lets : Lets d Γ₁ Γ₂} →
+    {prog : Com d Γ₂ t} →
+    {res : Σ (Γ₃ : Ctxt d.Ty), Lets d Γ₁ Γ₃ × Com d Γ₃ t × (t' : d.Ty) × Var Γ₃ t'} →
     (hres : res ∈ splitProgramAtAux pos lets prog) →
     (s : Valuation Γ₁) →
     res.2.2.1.denote (res.2.1.denote s) = prog.denote (lets.denote s)
@@ -1051,12 +1063,12 @@ theorem denote_splitProgramAtAux : {pos : ℕ} → {lets : Lets Op Γ₁ Γ₂} 
 with the `pos`th variable in `prog`, and an `Com` starting with the next variable.
 It also returns, the type of this variable and the variable itself as an element
 of the output `Ctxt` of the returned `Lets`.  -/
-def splitProgramAt (pos : ℕ) (prog : Com Op Γ₁ t) :
-    Option (Σ (Γ₂ : Ctxt Ty), Lets Op Γ₁ Γ₂ × Com Op Γ₂ t × (t' : Ty) × Var Γ₂ t') :=
+def splitProgramAt (pos : ℕ) (prog : Com d Γ₁ t) :
+    Option (Σ (Γ₂ : Ctxt d.Ty), Lets d Γ₁ Γ₂ × Com d Γ₂ t × (t' : d.Ty) × Var Γ₂ t') :=
   splitProgramAtAux pos .nil prog
 
-theorem denote_splitProgramAt {pos : ℕ} {prog : Com Op Γ₁ t}
-    {res : Σ (Γ₂ : Ctxt Ty), Lets Op Γ₁ Γ₂ × Com Op Γ₂ t × (t' : Ty) × Var Γ₂ t'}
+theorem denote_splitProgramAt {pos : ℕ} {prog : Com d Γ₁ t}
+    {res : Σ (Γ₂ : Ctxt d.Ty), Lets d Γ₁ Γ₂ × Com d Γ₂ t × (t' : d.Ty) × Var Γ₂ t'}
     (hres : res ∈ splitProgramAt pos prog) (s : Valuation Γ₁) :
     res.2.2.1.denote (res.2.1.denote s) = prog.denote s :=
   denote_splitProgramAtAux hres s
@@ -1071,10 +1083,10 @@ theorem denote_splitProgramAt {pos : ℕ} {prog : Com Op Γ₁ t}
 `target`. If it can match the variables, it inserts `rhs` into the program
 with the correct assignment of variables, and then replaces occurences
 of the variable at position `pos` in `target` with the output of `rhs`.  -/
-def rewriteAt (lhs rhs : Com Op Γ₁ t₁)
+def rewriteAt (lhs rhs : Com d Γ₁ t₁)
     (hlhs : ∀ t (v : Var Γ₁ t), ⟨t, v⟩ ∈ lhs.vars)
-    (pos : ℕ) (target : Com Op Γ₂ t₂) :
-    Option (Com Op Γ₂ t₂) := do
+    (pos : ℕ) (target : Com d Γ₂ t₂) :
+    Option (Com d Γ₂ t₂) := do
   let ⟨Γ₃, lets, target', t', vm⟩ ← splitProgramAt pos target
   if h : t₁ = t'
   then
@@ -1084,11 +1096,11 @@ def rewriteAt (lhs rhs : Com Op Γ₁ t₁)
     return addProgramInMiddle vm m lets (h ▸ rhs) target'
   else none
 
-theorem denote_rewriteAt (lhs rhs : Com Op Γ₁ t₁)
+theorem denote_rewriteAt (lhs rhs : Com d Γ₁ t₁)
     (hlhs : ∀ t (v : Var Γ₁ t), ⟨t, v⟩ ∈ lhs.vars)
-    (pos : ℕ) (target : Com Op Γ₂ t₂)
+    (pos : ℕ) (target : Com d Γ₂ t₂)
     (hl : lhs.denote = rhs.denote)
-    (rew : Com Op Γ₂ t₂)
+    (rew : Com d Γ₂ t₂)
     (hrew : rew ∈ rewriteAt lhs rhs hlhs pos target) :
     rew.denote = target.denote := by
   ext s
@@ -1115,18 +1127,18 @@ theorem denote_rewriteAt (lhs rhs : Com Op Γ₁ t₁)
       rintro rfl rfl
       simp
 
-variable (Op : _) {Ty : _} [OpSignature Op Ty] [TyDenote Ty] [OpDenote Op Ty] in
+variable (d : Dialect) [OpSignature d] [TyDenote d.Ty] [OpDenote d] in
 /--
   Rewrites are indexed with a concrete list of types, rather than an (erased) context, so that
   the required variable checks become decidable
 -/
-structure PeepholeRewrite (Γ : List Ty) (t : Ty) where
-  lhs : Com Op (.ofList Γ) t
-  rhs : Com Op (.ofList Γ) t
+structure PeepholeRewrite (Γ : List d.Ty) (t : d.Ty) where
+  lhs : Com d (.ofList Γ) t
+  rhs : Com d (.ofList Γ) t
   correct : lhs.denote = rhs.denote
 
-instance {Γ : List Ty} {t' : Ty} {lhs : Com Op (.ofList Γ) t'} :
-    Decidable (∀ (t : Ty) (v : Var (.ofList Γ) t), ⟨t, v⟩ ∈ lhs.vars) :=
+instance {Γ : List d.Ty} {t' : d.Ty} {lhs : Com d (.ofList Γ) t'} :
+    Decidable (∀ (t : d.Ty) (v : Var (.ofList Γ) t), ⟨t, v⟩ ∈ lhs.vars) :=
   decidable_of_iff
     (∀ (i : Fin Γ.length),
       let v : Var (.ofList Γ) (Γ.get i) := ⟨i, by simp [List.get?_eq_get, Ctxt.ofList]⟩
@@ -1141,9 +1153,9 @@ instance {Γ : List Ty} {t' : Ty} {lhs : Com Op (.ofList Γ) t'} :
   . intro h i
     apply h
 
-def rewritePeepholeAt (pr : PeepholeRewrite Op Γ t)
-    (pos : ℕ) (target : Com Op Γ₂ t₂) :
-    (Com Op Γ₂ t₂) := if hlhs : ∀ t (v : Var (.ofList Γ) t), ⟨_, v⟩ ∈ pr.lhs.vars then
+def rewritePeepholeAt (pr : PeepholeRewrite d Γ t)
+    (pos : ℕ) (target : Com d Γ₂ t₂) :
+    (Com d Γ₂ t₂) := if hlhs : ∀ t (v : Var (.ofList Γ) t), ⟨_, v⟩ ∈ pr.lhs.vars then
       match rewriteAt pr.lhs pr.rhs hlhs pos target
       with
         | some res => res
@@ -1151,8 +1163,8 @@ def rewritePeepholeAt (pr : PeepholeRewrite Op Γ t)
       else target
 
 
-theorem denote_rewritePeepholeAt (pr : PeepholeRewrite Op Γ t)
-    (pos : ℕ) (target : Com Op Γ₂ t₂) :
+theorem denote_rewritePeepholeAt (pr : PeepholeRewrite d Γ t)
+    (pos : ℕ) (target : Com d Γ₂ t₂) :
     (rewritePeepholeAt pr pos target).denote = target.denote := by
     simp only [rewritePeepholeAt]
     split_ifs
@@ -1168,8 +1180,8 @@ theorem denote_rewritePeepholeAt (pr : PeepholeRewrite Op Γ t)
 section SimpPeepholeApplier
 
 /-- rewrite with `pr` to `target` program, at location `ix` and later, running at most `fuel` steps. -/
-def rewritePeephole_go (fuel : ℕ) (pr : PeepholeRewrite Op Γ t)
-    (ix : ℕ) (target : Com Op Γ₂ t₂) : (Com Op Γ₂ t₂) :=
+def rewritePeephole_go (fuel : ℕ) (pr : PeepholeRewrite d Γ t)
+    (ix : ℕ) (target : Com d Γ₂ t₂) : (Com d Γ₂ t₂) :=
   match fuel with
   | 0 => target
   | fuel' + 1 =>
@@ -1178,12 +1190,12 @@ def rewritePeephole_go (fuel : ℕ) (pr : PeepholeRewrite Op Γ t)
 
 /-- rewrite with `pr` to `target` program, running at most `fuel` steps. -/
 def rewritePeephole (fuel : ℕ)
-    (pr : PeepholeRewrite Op Γ t) (target : Com Op Γ₂ t₂) : (Com Op Γ₂ t₂) :=
+    (pr : PeepholeRewrite d Γ t) (target : Com d Γ₂ t₂) : (Com d Γ₂ t₂) :=
   rewritePeephole_go fuel pr 0 target
 
 /-- `rewritePeephole_go` preserve semantics -/
-theorem denote_rewritePeephole_go (pr : PeepholeRewrite Op Γ t)
-    (pos : ℕ) (target : Com Op Γ₂ t₂) :
+theorem denote_rewritePeephole_go (pr : PeepholeRewrite d Γ t)
+    (pos : ℕ) (target : Com d Γ₂ t₂) :
     (rewritePeephole_go fuel pr pos target).denote = target.denote := by
   induction fuel generalizing pr pos target
   case zero =>
@@ -1193,7 +1205,7 @@ theorem denote_rewritePeephole_go (pr : PeepholeRewrite Op Γ t)
 
 /-- `rewritePeephole` preserves semantics. -/
 theorem denote_rewritePeephole (fuel : ℕ)
-    (pr : PeepholeRewrite Op Γ t) (target : Com Op Γ₂ t₂) :
+    (pr : PeepholeRewrite d Γ t) (target : Com d Γ₂ t₂) :
     (rewritePeephole fuel pr target).denote = target.denote := by
   simp[rewritePeephole, denote_rewritePeephole_go]
 end SimpPeepholeApplier
@@ -1202,11 +1214,11 @@ section Unfoldings
 
 /-- Equation lemma to unfold `denote`, which does not unfold correctly due to the presence
   of the coercion `ty_eq` and the mutual definition. -/
-theorem Expr.denote_unfold  [OP_SIG : OpSignature Op Ty] [OP_DENOTE: OpDenote Op Ty]
-    (op : Op)
+theorem Expr.denote_unfold  [OP_SIG : OpSignature d] [OP_DENOTE: OpDenote d]
+    (op : d.Op)
     (ty_eq : ty = OpSignature.outTy op)
     (args : HVector (Var Γ) <| OpSignature.sig op)
-    (regArgs : HVector (fun (t : Ctxt Ty × Ty) => Com Op t.1 t.2)
+    (regArgs : HVector (fun (t : Ctxt d.Ty × d.Ty) => Com d t.1 t.2)
       (OP_SIG.regSig op))
   : ∀(Γv : Γ.Valuation),
     Expr.denote (Expr.mk op ty_eq args regArgs) Γv =  ty_eq ▸ OP_DENOTE.denote op (args.map (fun _ v => Γv v)) regArgs.denote := by
@@ -1215,11 +1227,11 @@ theorem Expr.denote_unfold  [OP_SIG : OpSignature Op Ty] [OP_DENOTE: OpDenote Op
 
 /-- Equation lemma to unfold `denote`, which does not unfold correctly due to the presence
   of the coercion `ty_eq` and the mutual definition. -/
-theorem Com.denote_unfold  [OP_SIG : OpSignature Op Ty] [OP_DENOTE: OpDenote Op Ty]
-    (op : Op)
+theorem Com.denote_unfold  [OP_SIG : OpSignature d] [OP_DENOTE: OpDenote d]
+    (op : d.Op)
     (ty_eq : ty = OpSignature.outTy op)
     (args : HVector (Var Γ) <| OpSignature.sig op)
-    (regArgs : HVector (fun (t : Ctxt Ty × Ty) => Com Op t.1 t.2)
+    (regArgs : HVector (fun (t : Ctxt d.Ty × d.Ty) => Com d t.1 t.2)
       (OP_SIG.regSig op))
   : ∀(Γv : Γ.Valuation),
     Expr.denote (Expr.mk op ty_eq args regArgs) Γv =  ty_eq ▸ OP_DENOTE.denote op (args.map (fun _ v => Γv v)) regArgs.denote := by
@@ -1232,12 +1244,14 @@ end Unfoldings
 
 section TypeProjections
 
-def Com.getTy {Op Ty : Type} [OpSignature Op Ty] {Γ : Ctxt Ty} {t : Ty} : Com Op Γ t → Type := fun _ => Ty
-def Com.ty {Op Ty : Type} [OpSignature Op Ty] {Γ : Ctxt Ty} {t : Ty} : Com Op Γ t → Ty := fun _ => t
-def Com.ctxt {Op Ty : Type} [OpSignature Op Ty] {Γ : Ctxt Ty} {t : Ty} : Com Op Γ t → Ctxt Ty := fun _ => Γ
+variable {d} [OpSignature d] {Γ : Ctxt d.Ty} {t : d.Ty}
 
-def Expr.getTy {Op Ty : Type} [OpSignature Op Ty] {Γ : Ctxt Ty} {t : Ty} : Expr Op Γ t → Type := fun _ => Ty
-def Expr.ty {Op Ty : Type} [OpSignature Op Ty] {Γ : Ctxt Ty} {t : Ty} : Expr Op Γ t → Ty := fun _ => t
-def Expr.ctxt {Op Ty : Type} [OpSignature Op Ty] {Γ : Ctxt Ty} {t : Ty} : Expr Op Γ t → Ctxt Ty := fun _ => Γ
+def Com.getTy : Com d Γ t → Type      := fun _ => d.Ty
+def Com.ty    : Com d Γ t → d.Ty      := fun _ => t
+def Com.ctxt  : Com d Γ t → Ctxt d.Ty := fun _ => Γ
+
+def Expr.getTy  : Expr d Γ t → Type       := fun _ => d.Ty
+def Expr.ty     : Expr d Γ t → d.Ty       := fun _ => t
+def Expr.ctxt   : Expr d Γ t → Ctxt d.Ty  := fun _ => Γ
 
 end TypeProjections
